theories/lang/subst_map.v
@@ -1,17 +1,20 @@
 From stbor.lang Require Import expr_semantics.
 
-(** Substitution with a *map*, for the reflexivity proof. *)
-Fixpoint subst_map (xs : gmap string result) (e : expr) : expr :=
+Definition is_var {T: Type} (y: string) (x: string * T) :=
+  x.1 = y.
+Global Instance is_var_dec {T: Type} y x : Decision (@is_var T y x).
+Proof. rewrite /is_var /=. apply _. Qed.
+
+(** Substitution with a list of pairs instead of a pair of lists.
+This lets us do a total operation. *)
+Fixpoint subst_map (xs : list (string * result)) (e : expr) : expr :=
   match e with
-  | Var y => if xs !! y is Some v then of_result v else Var y
+  | Var y => if list_find (is_var y) xs is Some (_, (_, v)) then of_result v else Var y
   | Val v => Val v
-  (* | Rec f xl e =>
-    Rec f xl $ if bool_decide (BNamed x ≠ f ∧ BNamed x ∉ xl) then subst_map xs e else e *)
   | Call e el => Call (subst_map xs e) (map (subst_map xs) el)
   | InitCall e => InitCall (subst_map xs e)
   | EndCall e => EndCall (subst_map xs e)
   | Place l tag T => Place l tag T
-  (* | App e1 el => App (subst_map xs e1) (map (subst_map xs) el) *)
   | BinOp op e1 e2 => BinOp op (subst_map xs e1) (subst_map xs e2)
   | Proj e1 e2 => Proj (subst_map xs e1) (subst_map xs e2)
   | Conc e1 e2 => Conc (subst_map xs e1) (subst_map xs e2)
@@ -25,6 +28,55 @@ Fixpoint subst_map (xs : gmap string result) (e : expr) : expr :=
   | Let x1 e1 e2 =>
       Let x1
         (subst_map xs e1)
-        (subst_map (if x1 is BNamed s then delete s xs else xs) e2)
+        (subst_map (if x1 is BNamed s then list_filter (λ x, ¬is_var s x) _ xs else xs) e2)
   | Case e el => Case (subst_map xs e) (map (subst_map xs) el)
   end.
+
+Lemma subst_map_empty e :
+  subst_map [] e = e.
+Proof.
+  induction e; simpl; f_equal; eauto.
+  - admit.
+  - destruct x; done.
+  - admit.
+Admitted.
+
+Lemma subst_map_cons x rx xs e :
+  subst_map ((x,rx)::xs) e = subst_map xs (subst x rx e).
+Proof.
+  revert x rx xs; induction e; intros xx rx xs; try (simpl; f_equal; eauto).
+  - destruct (decide (x=xx)) as [<-|ne].
+    + rewrite decide_True //. rewrite bool_decide_true //.
+      destruct rx; done.
+    + rewrite decide_False. { intros ?. apply ne. done. }
+      rewrite bool_decide_false //.
+      simpl. destruct (list_find (is_var x) xs); last done.
+      simpl. destruct p as [? [? ?]]. done.
+  - admit.
+  - destruct x; simpl. done.
+    destruct (decide (s=xx)) as [<-|ne].
+    + rewrite decide_False //. { intros HH. apply HH. done. }
+      rewrite bool_decide_false //. intros ?. done.
+    + rewrite decide_True //. { intros ?. apply ne. done. }
+      rewrite bool_decide_true //. intros [= HH]. done.
+  - admit.
+Admitted.
+
+Definition fn_lists_to_subst {T: Type} (xbs : list binder) (xes : list T) :=
+  omap (λ '(x, e), if x is BNamed s then Some (s, e) else None) (zip xbs xes).
+
+Lemma subst_l_map (xbs : list binder) (xes : list value) (e es : expr) :
+  subst_l xbs (Val <$> xes) e = Some es →
+  es = subst_map (fn_lists_to_subst xbs (ValR <$> xes)) e.
+Proof.
+  revert xes es e; induction xbs; intros xes es e; destruct xes; try done.
+  - intros [= ->]. simpl.
+    by rewrite subst_map_empty.
+  - simpl.
+    set eo := subst_l _ _ _. destruct eo eqn:EQ; last done.
+    subst eo. intros [=<-].
+    specialize (IHxbs _ _ _ EQ).
+    destruct a.
+    + done.
+    + rewrite subst_map_cons. done.
+Qed.
